---
title: "Exploring the model"
format: pdf
---

## Quarto

## Equations

$$
H_i^0 \left( \frac{g_i}{m_i} - 1 \right) - S_\mu \, \bar{H} = (1 - \mu) H_i
$$

$$
H_i^0 \left( \frac{g_i}{m_i} - 1 \right) = (1 + S_\mu - \mu) \, \bar{H}
$$

$$
(1 - \mu) H_i = H_i^0 \left( \frac{g_i}{m_i} - 1 \right) - \frac{\mu}{1 + S_\mu - 1} \sum_j H_j^0 \left( \frac{g_j}{m_j} - 1 \right)
$$

$$
(1 - \mu) \, \text{NPP} = \sum_i \left[ m_i H_i^0 \left( \frac{g_i^2}{m_i^2} - \frac{g_i}{m_i} \right) \right] 
+ \frac{\mu}{1 + S_\mu - 1} \sum_i \sum_j \left[ m_i H_i^0 \left( \frac{g_i g_j}{m_i m_j} - \frac{g_i}{m_i} \right) H_i^0 H_j^0 \right]
$$

Define:

$$
\ast = m_i H_i^0 \left( \frac{g_i^2}{m_i^2} - \frac{g_i}{m_i} \right)
$$

Plugging in \( g_i \) on both sides and knowing that:

$$
\text{NPP} = \sum_i g_i H_i
$$

We get:

$$
(1 - \mu) \, \text{NPP} = \sum_i \ast - \frac{\mu}{1 + S_\mu - 1} \sum_{i,j} m_i H_i^0 \left( \frac{g_i g_j}{m_i m_j} - \frac{g_i}{m_i} \right) H_j^0
$$

Assuming:

$$
\sum_i S p_i = 1
$$

So \( p_i \, NPP \) in the sum is equal to NPP, where \( p \) is a vector.

Finally, with no competition \( \mu = 0 \), we have:

$$
\frac{g_i}{m_i} = 1 + \sqrt{\frac{4 p_i \, \text{NPP}}{F_i}}
$$

So you need:

$$
p_i \, \text{NPP} > \frac{F_i}{4}
$$

Where:

$$
F_i = m_i H_i^0
$$
